reasoning about the option monad.

theories/Monad/MonadLaws2.v
@@ -11,9 +11,9 @@ Section MonadLaws.
   Variable mleq : forall {T}, (T -> T -> Prop) -> m T -> m T -> Prop.
 
   Class MonadOrder : Type :=
-  { me_refl : forall T (e : T -> T -> Prop), 
+  { me_refl : forall T (e : T -> T -> Prop),
     Reflexive e -> Reflexive (mleq e)
-  ; me_trans : forall T (e : T -> T -> Prop), 
+  ; me_trans : forall T (e : T -> T -> Prop),
     Transitive e -> Transitive (mleq e)
   }.
 
@@ -37,15 +37,20 @@ Section MonadLaws.
   Proof.
     split; unfold meq in *; intuition; eapply me_trans; try eassumption.
   Qed.
-    
+
+  (** TODO: The real question is whether all of these [eX] relations
+   ** need to be reflexive and transitive. They don't seem to need to be
+   ** for option monad, but the proofs would be more automatable if they
+   ** were b/c I'd be able to rewrite.
+   **)
   Class MonadLaws : Type :=
-  { morder :> MonadOrder 
+  { morder :> MonadOrder
   ; bind_of_return : forall A B (a:A) (f:A -> m B) (eB : B -> B -> Prop),
     meq eB (bind (ret a) f) (f a)
   ; return_of_bind : forall A (aM:m A) (f:A -> m A) (eA : A -> A -> Prop),
     Reflexive eA ->
     (forall x, meq eA (f x) (ret x)) -> meq eA (bind aM f) aM
-  ; bind_associativity : 
+  ; bind_associativity :
     forall A B C (aM:m A) (f:A -> m B) (g:B -> m C) (eC : C -> C -> Prop),
       Reflexive eC -> Transitive eC ->
       meq eC (bind (bind aM f) g) (bind aM (fun a => bind (f a) g))
@@ -76,28 +81,32 @@ Section MonadLaws.
     intros; intuition. split; eapply bind_parametric_tl_leq; eauto; intros; edestruct H0; eauto.
   Qed.
 
-(*
   Class MonadTLaws (n : Type -> Type) (nM : Monad n) (MT : MonadT m n) : Type :=
-  { lift_ret  : forall T (x : T), meq (lift (ret x)) (ret x)
-  ; lift_bind : forall T U (c : n T) (f : T -> n U), meq (lift (bind c f)) (bind (lift c) (fun x => lift (f x)))
+  { lift_ret  : forall T (x : T) (eT : T -> T -> Prop),
+    Reflexive eT -> Transitive eT ->
+    meq eT (lift (ret x)) (ret x)
+  ; lift_bind : forall T U (c : n T) (f : T -> n U) (eU : U -> U -> Prop),
+    Reflexive eU -> Transitive eU ->
+    meq eU (lift (bind c f)) (bind (lift c) (fun x => lift (f x)))
   }.
 
+(*
   Class MonadStateLaws s (MS : State s m) : Type :=
   { get_put : meq (bind get put) (ret tt)
   }.
 
   Class MonadReaderLaws S (MS : Reader S m) : Type :=
   { ask_local : forall f, meq (local f ask) (bind ask (fun x => ret (f x)))
-  ; local_local : forall T (s s' : S -> S) (c : m T), 
+  ; local_local : forall T (s s' : S -> S) (c : m T),
     meq (local s (local s' c)) (local (fun x => s' (s x)) c)
   }.
 
   Class MonadZeroLaws (MZ : Zero m) : Type :=
-  { bind_zero : 
+  { bind_zero :
     forall A B c, meq (@bind _ M _ (@zero _ _ A) _ c) (@zero _ _ B)
   }.
 
-  Class MonadFixLaws (MF : MonadFix m) (leq : forall {T}, m T -> m T -> Prop) 
+  Class MonadFixLaws (MF : MonadFix m) (leq : forall {T}, m T -> m T -> Prop)
     : Type :=
   { leq_refl : forall T, Reflexive (@leq T)
   ; leq_trans : forall T, Transitive (@leq T)
@@ -108,17 +117,16 @@ Section MonadLaws.
 
 End MonadLaws.
 
-(*
 Hint Rewrite bind_of_return bind_associativity using (eauto with typeclass_instances) : monad_rw.
 (* Hint Rewrite lift_ret lift_bind get_put ask_local local_local bind_zero : monad_rw. *)
 
 Ltac monad_norm :=
-  let tac := 
-    repeat (rewrite bind_parametric_hd; [ eassumption | eauto with typeclass_instances | intros ]); 
-    repeat (rewrite bind_parametric_tl; [ reflexivity | eauto with typeclass_instances | intros ]); 
-    repeat (rewrite return_of_bind; [ solve [ eauto ] | eauto with typeclass_instances | intros ]); 
+  let tc := solve [ eauto with typeclass_instances ] in
+  let tac :=
+    repeat (eapply bind_parametric_hd; [ tc | tc | ]);
+    repeat (eapply bind_parametric_tl; [ tc | tc | intros ]);
+    repeat (rewrite return_of_bind; [ tc | tc | intros ]);
     try (autorewrite with monad_rw; intros)
   in
   try ( unfold liftM, liftM2 in * ) ;
   repeat progress tac.
-*)
